theories/util/proof_irrelevance.v
@@ -1,0 +1,4 @@
+Require Import ssreflect ProofIrrelevance.
+
+Ltac proof_subst x y :=
+  (have ?: x = y by apply proof_irrelevance); subst x.
